CapFlex.v

src/prop/Mapping.v
@@ -3211,3 +3211,242 @@ Section SHIFTMAP.
   Qed.
 
 End SHIFTMAP.
+
+Section CONCRETEIDENT.
+
+  Definition map_ident_concrete (f: Loc.t -> Time.t -> Time.t -> Prop)
+             (mem: Memory.t): Prop :=
+    forall loc to
+           (CONCRETE: concrete_promised mem loc to),
+      f loc to to.
+
+  Definition map_ident_concrete_bot
+             f mem
+             (MAP: map_ident_concrete f mem)
+             (CLOSED: Memory.closed mem)
+    :
+      mapping_map_bot f.
+  Proof.
+    ii. eapply MAP. inv CLOSED. econs; eauto.
+  Qed.
+
+  Lemma map_ident_concrete_closed_timemap
+        f mem tm
+        (MAP: map_ident_concrete f mem)
+        (CLOSED: Memory.closed_timemap tm mem)
+    :
+      timemap_map f tm tm.
+  Proof.
+    ii. eapply MAP; eauto.
+    exploit CLOSED; eauto. i. des. econs; eauto.
+  Qed.
+
+  Lemma map_ident_concrete_closed_view
+        f mem vw
+        (MAP: map_ident_concrete f mem)
+        (CLOSED: Memory.closed_view vw mem)
+    :
+      view_map f vw vw.
+  Proof.
+    inv CLOSED. econs.
+    - eapply map_ident_concrete_closed_timemap; eauto.
+    - eapply map_ident_concrete_closed_timemap; eauto.
+  Qed.
+
+  Lemma map_ident_concrete_closed_tview
+        f mem tvw
+        (MAP: map_ident_concrete f mem)
+        (CLOSED: TView.closed tvw mem)
+    :
+      tview_map f tvw tvw.
+  Proof.
+    inv CLOSED. econs.
+    - i. eapply map_ident_concrete_closed_view; eauto.
+    - eapply map_ident_concrete_closed_view; eauto.
+    - eapply map_ident_concrete_closed_view; eauto.
+  Qed.
+
+  Lemma map_ident_concrete_closed_opt_view
+        f mem vw
+        (MAP: map_ident_concrete f mem)
+        (CLOSED: Memory.closed_opt_view vw mem)
+    :
+      opt_view_map f vw vw.
+  Proof.
+    inv CLOSED; econs.
+    eapply map_ident_concrete_closed_view; eauto.
+  Qed.
+
+  Lemma map_ident_concrete_closed_message
+        f mem msg
+        (MAP: map_ident_concrete f mem)
+        (CLOSED: Memory.closed_message msg mem)
+    :
+      msg_map f msg msg.
+  Proof.
+    inv CLOSED; econs.
+    eapply map_ident_concrete_closed_opt_view; eauto.
+  Qed.
+
+  Inductive compose_map (f0 f1: Loc.t -> Time.t -> Time.t -> Prop)
+    : Loc.t -> Time.t -> Time.t -> Prop :=
+  | compose_map_intro
+      loc ts0 ts1 ts2
+      (MAP0: f0 loc ts0 ts1)
+      (MAP1: f1 loc ts1 ts2)
+    :
+      compose_map f0 f1 loc ts0 ts2
+  .
+  Hint Constructors compose_map.
+
+  Lemma compose_map_eq f0 f1
+        (MAPEQ0: mapping_map_eq f0)
+        (MAPEQ1: mapping_map_eq f1)
+    :
+      mapping_map_eq (compose_map f0 f1).
+  Proof.
+    unfold mapping_map_eq in *. i. inv MAP0. inv MAP1.
+    hexploit (@MAPEQ0 _ _ _ _ MAP2 MAP0); eauto. i. clarify.
+    eauto.
+  Qed.
+
+  Lemma compose_map_le f0 f1
+        (MAPLE0: mapping_map_le f0)
+        (MAPLE1: mapping_map_le f1)
+    :
+      mapping_map_le (compose_map f0 f1).
+  Proof.
+    unfold mapping_map_le in *. i. inv MAP0. inv MAP1.
+    hexploit (@MAPLE0 _ _ _ _ _ MAP2 MAP0); eauto.
+  Qed.
+
+  Lemma compose_map_bot f0 f1
+        (MAPBOT0: mapping_map_bot f0)
+        (MAPBOT1: mapping_map_bot f1)
+    :
+      mapping_map_bot (compose_map f0 f1).
+  Proof.
+    ii. econs; eauto.
+  Qed.
+
+  Lemma compose_map_lt f0 f1
+        (MAPLT0: mapping_map_lt f0)
+        (MAPLT1: mapping_map_lt f1)
+    :
+      mapping_map_lt (compose_map f0 f1).
+  Proof.
+    unfold mapping_map_lt in *. i. inv MAP0. inv MAP1.
+    transitivity (Time.lt ts1 ts2); eauto.
+  Qed.
+
+  Lemma compose_map_timemap f0 f1 tm0 tm1 tm2
+        (MAP0: timemap_map f0 tm0 tm1)
+        (MAP1: timemap_map f1 tm1 tm2)
+    :
+      timemap_map (compose_map f0 f1) tm0 tm2.
+  Proof.
+    ii. eauto.
+  Qed.
+
+  Lemma compose_map_view f0 f1 vw0 vw1 vw2
+        (MAP0: view_map f0 vw0 vw1)
+        (MAP1: view_map f1 vw1 vw2)
+    :
+      view_map (compose_map f0 f1) vw0 vw2.
+  Proof.
+    inv MAP0. inv MAP1. econs.
+    - eapply compose_map_timemap; eauto.
+    - eapply compose_map_timemap; eauto.
+  Qed.
+
+  Lemma compose_map_opt_view f0 f1 vw0 vw1 vw2
+        (MAP0: opt_view_map f0 vw0 vw1)
+        (MAP1: opt_view_map f1 vw1 vw2)
+    :
+      opt_view_map (compose_map f0 f1) vw0 vw2.
+  Proof.
+    inv MAP0; inv MAP1; econs.
+    eapply compose_map_view; eauto.
+  Qed.
+
+  Lemma compose_map_tview f0 f1 tvw0 tvw1 tvw2
+        (MAP0: tview_map f0 tvw0 tvw1)
+        (MAP1: tview_map f1 tvw1 tvw2)
+    :
+      tview_map (compose_map f0 f1) tvw0 tvw2.
+  Proof.
+    inv MAP0. inv MAP1. econs.
+    - i. eapply compose_map_view; eauto.
+    - eapply compose_map_view; eauto.
+    - eapply compose_map_view; eauto.
+  Qed.
+
+  Lemma compose_map_msg f0 f1 msg0 msg1 msg2
+        (MAP0: msg_map f0 msg0 msg1)
+        (MAP1: msg_map f1 msg1 msg2)
+    :
+      msg_map (compose_map f0 f1) msg0 msg2.
+  Proof.
+    inv MAP0; inv MAP1; econs.
+    eapply compose_map_opt_view; eauto.
+  Qed.
+
+  Lemma compose_map_mappable f0 f1 mem0 mem1
+        (MAP: memory_map f0 mem0 mem1)
+        (MAPPABLE: mappable_memory f1 mem1)
+    :
+      mappable_memory (compose_map f0 f1) mem0.
+  Proof.
+    ii. inv MAP. exploit MAPPED; eauto. i. des; clarify.
+    inv MSG. inv MSGLE. exploit MAPPABLE; eauto. i. inv x.
+    eexists. eauto.
+  Qed.
+
+  Lemma compose_map_memory2 f0 f1 m0 m1 m2
+        (MAPEQ0: mapping_map_eq f0)
+        (MAPLE: mapping_map_le f1)
+        (MEM0: memory_map2 f0 m0 m1)
+        (CLOSED0: Memory.closed m0)
+        (MEM1: memory_map2 f1 m1 m2)
+    :
+      memory_map2 (compose_map f0 f1) m0 m2.
+  Proof.
+    dup MEM0. dup MEM1.
+    inv MEM0. inv MEM1. econs.
+    - ii. exploit MAPPED; eauto. i. des; auto.
+      exploit MAPPED0; eauto. i. des; auto.
+      + subst. inv MSGLE. inv MSG. auto.
+      + right. inv CLOSED0. exploit CLOSED; eauto. i. des.
+        exploit closed_message_map; try apply MSG; eauto.
+        { eapply memory_map2_memory_map; eauto. } intros MSG_CLOSED1.
+        exploit msg_map_exists; try apply MSG_CLSOED1; eauto.
+        { eapply memory_map2_memory_map; eauto. } i. des.
+        esplits; [..|eauto].
+        * eauto.
+        * eapply compose_map_msg; eauto.
+        * etrans; eauto. eapply msg_le_map; eauto.
+    - i. exploit ONLY0; eauto. i. des.
+      exploit ONLY; eauto. i. des. esplits; eauto.
+  Qed.
+
+  Lemma compose_map_promise f0 f1 m0 m1 m2
+        (MAPLT0: mapping_map_lt f0)
+        (MAPLT1: mapping_map_lt f1)
+        (MEM0: promises_map f0 m0 m1)
+        (CLOSED0: Memory.closed m0)
+        (MEM1: promises_map f1 m1 m2)
+    :
+      promises_map (compose_map f0 f1) m0 m2.
+  Proof.
+    dup MEM0. dup MEM1.
+    inv MEM0. inv MEM1. econs.
+    - ii. exploit MAPPED; eauto. i. des; auto.
+      exploit MAPPED0; eauto. i. des; auto. esplits; eauto.
+      + eapply mapping_map_lt_non_collapsable.
+        eapply compose_map_lt; eauto.
+      + eapply compose_map_msg; eauto.
+    - ii. exploit ONLY0; eauto. i. des.
+      exploit ONLY; eauto. i. des. esplits; eauto.
+  Qed.
+
+End CONCRETEIDENT.
