src/prop/CapFlex.v
@@ -1,0 +1,483 @@
+Require Import RelationClasses.
+
+From Paco Require Import paco.
+From sflib Require Import sflib.
+
+From PromisingLib Require Import Axioms.
+From PromisingLib Require Import Basic.
+From PromisingLib Require Import DataStructure.
+From PromisingLib Require Import Language.
+From PromisingLib Require Import Loc.
+Require Import Time.
+Require Import Event.
+Require Import View.
+Require Import Cell.
+Require Import Memory.
+Require Import MemoryFacts.
+Require Import TView.
+Require Import Local.
+Require Import Thread.
+Require Import Configuration.
+Require Import Progress.
+Require Import Behavior.
+Require Import Cover.
+Require Import Pred.
+Require Import Trace.
+
+Require Import MemoryProps.
+Require Import Mapping.
+
+Set Implicit Arguments.
+
+Section CAPFLEX.
+
+  Record cap_flex (mem1 mem2: Memory.t) (tm: TimeMap.t): Prop :=
+    {
+      cap_flex_le: Memory.le mem1 mem2;
+      cap_flex_middle: forall loc from1 to1 from2 to2
+                              (ADJ: Memory.adjacent loc from1 to1 from2 to2 mem1)
+                              (TO: Time.lt to1 from2),
+          Memory.get loc from2 mem2 = Some (to1, Message.reserve);
+      cap_flex_back: forall loc, Memory.get loc (tm loc) mem2 =
+                                 Some (Memory.max_ts loc mem1, Message.reserve);
+      cap_flex_complete: forall loc from to msg
+                               (GET1: Memory.get loc to mem1 = None)
+                               (GET2: Memory.get loc to mem2 = Some (from, msg)),
+          (exists f m, Memory.get loc from mem1 = Some (f, m));
+    }
+  .
+
+  Lemma cap_flex_inv
+        mem1 mem2 tm
+        loc from to msg
+        (CLOSED: Memory.closed mem1)
+        (CAP: cap_flex mem1 mem2 tm)
+        (GET: Memory.get loc to mem2 = Some (from, msg))
+        (TM: forall loc, Time.lt (Memory.max_ts loc mem1) (tm loc))
+    :
+    Memory.get loc to mem1 = Some (from, msg) \/
+    (Memory.get loc to mem1 = None /\
+     exists from1 to2,
+        Memory.adjacent loc from1 from to to2 mem1 /\
+        Time.lt from to /\
+        msg = Message.reserve) \/
+    (Memory.get loc to mem1 = None /\
+     from = Memory.max_ts loc mem1 /\
+     to = tm loc /\
+     msg = Message.reserve).
+  Proof.
+    inv CAP. move GET at bottom.
+    destruct (Memory.get loc to mem1) as [[]|] eqn:GET1.
+    { exploit cap_flex_le0; eauto. i.
+      rewrite GET in x. inv x. auto. }
+    right. exploit cap_flex_complete0; eauto. i. des.
+    exploit Memory.max_ts_spec; eauto. i. des. inv MAX.
+    - left.
+      exploit Memory.adjacent_exists; try eapply H; eauto. i. des.
+      assert (LT: Time.lt from from2).
+      { clear cap_flex_middle0 cap_flex_back0 cap_flex_complete0 GET0 H.
+        (* clear MIDDLE BACK COMPLETE GET0 H. *)
+        inv x1. rewrite GET0 in x. inv x.
+        exploit Memory.get_ts; try exact GET2. i. des.
+        { subst. inv TS. }
+        destruct (Time.le_lt_dec from2 from); auto.
+        inv l.
+        - exfalso.
+          exploit Memory.get_ts; try exact GET0. i. des.
+          { subst. inv H. }
+          exploit Memory.get_disjoint; [exact GET0|exact GET2|..]. i. des.
+          { subst. timetac. }
+          apply (x2 from); econs; ss.
+          + refl.
+          + econs. auto.
+        - exfalso. inv H.
+          exploit cap_flex_le0; try exact GET2. i.
+          exploit Memory.get_ts; try exact GET. i. des.
+          { subst. rewrite GET1 in GET0. inv GET0. }
+          exploit Memory.get_disjoint; [exact GET|exact x|..]. i. des.
+          { subst. rewrite GET1 in GET2. inv GET2. }
+          destruct (Time.le_lt_dec to to2).
+          + apply (x3 to); econs; ss. refl.
+          + apply (x3 to2); econs; ss.
+            * econs. auto.
+            * refl.
+      }
+      exploit cap_flex_middle0; try eapply x1; eauto. i.
+      destruct (Time.eq_dec to from2).
+      + subst. rewrite GET in x0. inv x0. esplits; eauto.
+      + exfalso. inv x1.
+        exploit Memory.get_ts; try exact GET. i. des.
+        { subst. rewrite GET1 in x. inv x. }
+        exploit Memory.get_ts; try exact x0. i. des.
+        { subst. exploit cap_flex_le0; try exact GET3. i.
+          exploit Memory.get_disjoint; [exact GET|exact x1|..]. i. des.
+          { subst. rewrite GET1 in GET3. inv GET3. }
+          destruct (Time.le_lt_dec to to2).
+          - apply (x4 to); econs; ss. refl.
+          - apply (x4 to2); econs; ss.
+            + econs. auto.
+            + refl.
+        }
+        exploit Memory.get_disjoint; [exact GET|exact x0|..]. i. des; try congr.
+        destruct (Time.le_lt_dec to from2).
+        * apply (x4 to); econs; ss. refl.
+        * apply (x4 from2); econs; ss.
+          { econs. auto. }
+          { refl. }
+    - right. inv H. do 2 (split; auto).
+      rewrite GET0 in x. inv x.
+      specialize (cap_flex_back0 loc).
+      exploit Memory.get_ts; try exact GET. i. des; try congr.
+      exploit Memory.get_disjoint; [exact GET|exact cap_flex_back0|..]. i. des.
+      { subst. esplits; eauto. }
+      exfalso.
+      destruct (Time.le_lt_dec to (tm loc)).
+      + apply (x1 to); econs; ss. refl.
+      + apply (x1 (tm loc)); econs; s;
+          eauto using TM; try refl.
+        econs. ss.
+  Qed.
+
+  Lemma cap_flex_exists
+        mem1 tm
+        (CLOSED1: Memory.closed mem1)
+        (TM: forall loc, Time.lt (Memory.max_ts loc mem1) (tm loc))
+    :
+      exists mem2, (<<CAP: cap_flex mem1 mem2 tm>>).
+  Proof.
+    hexploit Memory.cap_exists; eauto. i. des.
+    hexploit (@choice
+                Loc.t Cell.t
+                (fun loc cell =>
+                   forall ts,
+                     Cell.get ts cell =
+                     if (Time.eq_dec ts (tm loc))
+                     then Some (Memory.max_ts loc mem1, Message.reserve)
+                     else if (Time.eq_dec ts (Time.incr (Memory.max_ts loc mem1)))
+                          then None
+                          else Memory.get loc ts mem2)).
+    { intros loc.
+      hexploit (@Cell.remove_exists (mem2 loc)).
+      { inv CAP. eapply BACK. } i. des.
+      hexploit (@Cell.add_exists cell2 (Memory.max_ts loc mem1) (tm loc) Message.reserve).
+      { i. erewrite Cell.remove_o in GET2; eauto. des_ifs.
+        eapply Memory.cap_inv in GET2; eauto. des; clarify.
+        { symmetry. eapply interval_le_disjoint.
+          eapply Memory.max_ts_spec in GET2. des. auto. }
+        { inv GET0. symmetry. eapply interval_le_disjoint.
+          transitivity to0.
+          { eapply memory_get_ts_le; eauto. }
+          { eapply Memory.max_ts_spec in GET4. des. auto. }
+        }
+      }
+      { eauto. }
+      { econs. } i. des.
+      exists cell0. i.
+      erewrite Cell.add_o; eauto. erewrite Cell.remove_o; eauto. des_ifs. }
+    intros [mem3 SPEC].
+
+    exists mem3. dup CAP. inv CAP. econs.
+    { ii. unfold Memory.get. rewrite SPEC. des_ifs.
+      { eapply Memory.max_ts_spec in LHS. des.
+        exfalso. eapply Time.lt_strorder. eapply TimeFacts.lt_le_lt.
+        { eapply TM. }
+        { eapply MAX. }
+      }
+      { eapply Memory.max_ts_spec in LHS. des.
+        exfalso. eapply Time.lt_strorder. eapply TimeFacts.lt_le_lt.
+        { eapply Time.incr_spec. }
+        { eapply MAX. }
+      }
+      { eapply SOUND; auto. }
+    }
+    { i. unfold Memory.get. erewrite SPEC. dup ADJ. inv ADJ. des_ifs.
+      { dup GET2. apply Memory.max_ts_spec in GET2. des.
+        apply Memory.get_ts in GET0. des; subst.
+        { exfalso. eapply Time.lt_strorder. eapply TimeFacts.lt_le_lt.
+          { eapply TS. }
+          { eapply Time.bot_spec. }
+        }
+        { exfalso. eapply Time.lt_strorder. eapply TimeFacts.lt_le_lt.
+          { eapply GET0. } etrans.
+          { eapply MAX. }
+          { left. eauto. }
+        }
+      }
+      { dup GET2. apply Memory.max_ts_spec in GET2. des.
+        apply Memory.get_ts in GET0. des; subst.
+        { exfalso. eapply Time.lt_strorder. eapply TimeFacts.lt_le_lt.
+          { eapply TS. }
+          { eapply Time.bot_spec. }
+        }
+        { exfalso. eapply Time.lt_strorder. eapply TimeFacts.lt_le_lt.
+          { eapply GET0. } etrans.
+          { eapply MAX. }
+          { left. eapply Time.incr_spec. }
+        }
+      }
+      { eapply MIDDLE; eauto. }
+    }
+    { i. unfold Memory.get. erewrite SPEC. des_ifs. }
+    { i. unfold Memory.get in GET2. rewrite SPEC in GET2. des_ifs.
+      { hexploit (@Memory.max_ts_spec loc).
+        { inv CLOSED1. eapply INHABITED. }
+        i. des. eauto. }
+      { eapply COMPLETE; eauto. }
+    }
+  Qed.
+
+  Lemma cap_cap_flex mem1 mem2
+        (CAP: Memory.cap mem1 mem2)
+    :
+      cap_flex mem1 mem2 (fun loc => Time.incr (Memory.max_ts loc mem1)).
+  Proof.
+    inv CAP. econs; eauto.
+  Qed.
+
+  Lemma cap_flex_max_ts mem1 mem2 tm
+        (CLOSED: Memory.closed mem1)
+        (CAP: cap_flex mem1 mem2 tm)
+        (TM: forall loc, Time.lt (Memory.max_ts loc mem1) (tm loc))
+    :
+      forall loc,
+        Memory.max_ts loc mem2 = tm loc.
+  Proof.
+    i. set (BACK:=CAP.(cap_flex_back) loc).
+    exploit Memory.max_ts_spec; try exact BACK. i. des.
+    apply TimeFacts.antisym; ss.
+    destruct (Time.le_lt_dec (Memory.max_ts loc mem2) (tm loc)); ss.
+    exploit cap_flex_inv; try exact GET; eauto. i. des.
+    - exploit Memory.max_ts_spec; try exact x0. i. des.
+      exploit TimeFacts.lt_le_lt; try exact l; try exact MAX0. i.
+      specialize (TM loc). rewrite x1 in TM. timetac.
+    - inv x1. exploit Memory.get_ts; try exact GET2. i. des.
+      { rewrite x1 in *. inv l. }
+      exploit Memory.max_ts_spec; try exact GET2. i. des.
+      exploit TimeFacts.lt_le_lt; try exact x1; try exact MAX0. i.
+      rewrite x3 in l. specialize (TM loc). rewrite l in TM. timetac.
+    - subst. rewrite x2 in *. timetac.
+  Qed.
+
+  Lemma cap_flex_covered
+        mem0 mem1 tm
+        (CAP: cap_flex mem0 mem1 tm)
+        (CLOSED: Memory.closed mem0)
+        (TM: forall loc, Time.lt (Memory.max_ts loc mem0) (tm loc))
+        loc to
+    :
+      Interval.mem (Time.bot, (tm loc)) to
+      <->
+      covered loc to mem1.
+  Proof.
+    split; i.
+    {
+      inv H. set (@cell_elements_least
+                             (mem0 loc)
+                             (fun to' => Time.le to to')). des; cycle 1.
+      { destruct (Time.le_lt_dec to (Memory.max_ts loc mem0)).
+        - exfalso. exploit Memory.max_ts_spec.
+          + eapply CLOSED.
+          + i. des. exploit EMPTY; eauto.
+        - econs.
+          + eapply cap_flex_back; eauto.
+          + econs; eauto. }
+      set (@cell_elements_greatest
+             (mem0 loc)
+             (fun to' => Time.lt to' to)). des; cycle 1.
+      { exfalso. exploit EMPTY.
+        - eapply CLOSED.
+        - eauto.
+        - ss. }
+      destruct (Time.le_lt_dec to from).
+      - exploit CAP.(cap_flex_middle).
+        + econs.
+          * eapply GET0.
+          * eapply GET.
+          * eapply TimeFacts.lt_le_lt; eauto.
+          * i. destruct (Memory.get loc ts mem0) eqn:GET1; auto.
+            exfalso. destruct p.
+            destruct (Time.le_lt_dec to ts).
+            { exploit LEAST; eauto. i.
+              eapply Time.lt_strorder. eapply TimeFacts.le_lt_lt.
+              { eapply x. }
+              eapply TimeFacts.le_lt_lt.
+              { eapply TS2. }
+              { eapply memory_get_ts_strong in GET. des; clarify; ss.
+                exfalso. eapply Time.lt_strorder. eapply TimeFacts.le_lt_lt.
+                - eapply l.
+                - eauto. } }
+            { exploit GREATEST; eauto. i.
+              eapply Time.lt_strorder. eapply TimeFacts.le_lt_lt.
+              { eapply x. }
+              { eauto. } }
+        + eapply TimeFacts.lt_le_lt; eauto.
+        + i. econs; eauto. econs; eauto.
+      - econs.
+        + eapply CAP.(cap_flex_le). eapply GET.
+        + econs; eauto.
+    }
+    {
+      inv H. apply Memory.max_ts_spec in GET. des.
+      inv ITV. ss. econs; ss.
+      - eapply TimeFacts.le_lt_lt; eauto. apply Time.bot_spec.
+      - etrans; eauto. erewrite <- cap_flex_max_ts; eauto.
+    }
+  Qed.
+
+  Record cap_flex_map (max tm0 tm1: TimeMap.t)
+         (times: Loc.t -> list Time.t)
+         (f: Loc.t -> Time.t -> Time.t -> Prop): Prop :=
+    {
+      cap_flex_map_map_lt:
+        mapping_map_lt f;
+      cap_flex_map_map_bot:
+        mapping_map_bot f;
+      cap_flex_map_ident:
+        forall loc ts (TS: Time.le ts (max loc)),
+          f loc ts ts;
+      cap_flex_map_max:
+        forall loc,
+        exists fts,
+          (<<MAP: f loc (tm0 loc) fts>>) /\
+          (<<TS: Time.le (tm1 loc) fts>>);
+      cap_flex_map_complete:
+        forall loc ts (IN: List.In ts (times loc)),
+          mappable_time f loc ts;
+    }.
+
+  Lemma cap_flex_map_exists max tm0 tm1 times
+        (TM0: forall loc, Time.lt (max loc) (tm0 loc))
+        (TM1: forall loc, Time.lt (max loc) (tm1 loc))
+    :
+      exists f,
+        (<<MAP: cap_flex_map max tm0 tm1 times f>>).
+  Proof.
+    hexploit (@choice
+                Loc.t (Time.t -> Time.t -> Prop)
+                (fun loc f =>
+                   (<<MAPLT: mapping_map_lt_loc f>>) /\
+                   (<<IDENT: forall ts (TS: Time.le ts (max loc)),
+                       f ts ts>>) /\
+                   (<<MAX: exists fts,
+                       (<<MAP: f (tm0 loc) fts>>) /\
+                       (<<TS: Time.le (tm1 loc) fts>>)>>)/\
+                   (<<COMPLETE: forall ts (IN: List.In ts (times loc)),
+                       exists fts, (<<MAP: f ts fts>>)>>))).
+    { intros loc.
+      hexploit (@shift_map_exists
+                  (max loc) (tm1 loc) (Time.incr (tm1 loc))
+                  ((tm0 loc)::times loc)); ss.
+      { left. auto. }
+      { apply Time.incr_spec. }
+      intros [f SPEC]. exists f. des. splits; auto.
+      { hexploit (COMPLETE (tm0 loc)); eauto. i. des. esplits; eauto.
+        eapply BOUND in MAPPED; eauto. left. des. auto. }
+      { i. hexploit (COMPLETE ts); eauto. }
+    }
+    intros [f SPEC]. exists f. econs.
+    { eapply mapping_map_lt_locwise.
+      i. specialize (SPEC loc). des. auto. }
+    { ii. specialize (SPEC loc). des.
+      eapply IDENT. eapply Time.bot_spec. }
+    { i. specialize (SPEC loc). des. auto. }
+    { i. specialize (SPEC loc). des. eauto. }
+    { i. specialize (SPEC loc). des.
+      exploit COMPLETE; eauto. }
+  Qed.
+
+  Lemma concrete_messages_le_cap_flex_memory_map
+        mem0 mem1 tm0 tm1 cap0 cap1 times f
+        (CONCRETE: concrete_messages_le mem0 mem1)
+        (TM0: forall loc, Time.lt (Memory.max_ts loc mem0) (tm0 loc))
+        (TM1: forall loc, Time.lt (Memory.max_ts loc mem1) (tm1 loc))
+        (CAP0: cap_flex mem0 cap0 tm0)
+        (CAP1: cap_flex mem1 cap1 tm1)
+        (MEM0: Memory.closed mem0)
+        (MEM1: Memory.closed mem1)
+        (MAP: cap_flex_map (Memory.max_timemap mem0) tm0 tm1 times f)
+    :
+      memory_map f cap0 cap1.
+  Proof.
+    assert (IDENT: map_ident_in_memory f mem0).
+    { ii. eapply cap_flex_map_ident; eauto. }
+    econs.
+    { i. eapply (@cap_flex_inv mem0 cap0 tm0) in GET; eauto. des; eauto.
+      destruct msg as [val released|]; auto. right.
+      exploit CONCRETE; eauto. i. des. esplits.
+      { eapply cap_flex_map_ident; eauto.
+        eapply Memory.max_ts_spec in GET. des. auto. }
+      { eapply map_ident_in_memory_closed_message; eauto.
+        eapply MEM0 in GET. des; auto. }
+      { refl. }
+      { eapply CAP1.(cap_flex_le) in GET1. eauto. }
+    }
+    { i. hexploit (MAP.(cap_flex_map_max) loc). i. des.
+      left. exists (tm0 loc), Time.bot, fts, Time.bot. splits; auto.
+      { eapply Time.bot_spec. }
+      { hexploit (@cap_flex_max_ts mem1 cap1 tm1); eauto.
+        i. eapply Memory.max_ts_spec in GET. des.
+        erewrite H in MAX. etrans; eauto. }
+      { eapply MAP.(cap_flex_map_map_bot). }
+      { i. eapply cap_flex_covered; eauto. }
+    }
+  Qed.
+
+  Lemma cap_flex_closed mem cap tm
+        (CAP: cap_flex mem cap tm)
+        (TM: forall loc, Time.lt (Memory.max_ts loc mem) (tm loc))
+        (CLOSED: Memory.closed mem)
+    :
+      Memory.closed cap.
+  Proof.
+    dup CLOSED. inv CLOSED. econs.
+    { i. eapply cap_flex_inv in MSG; eauto. des; subst.
+      { exploit CLOSED1; eauto. i. des. splits; auto.
+        eapply concrete_promised_le_closed_message; eauto.
+        eapply concrete_messages_le_concrete_promised_le; eauto.
+        eapply memory_le_concrete_messages_le; eauto.
+        eapply cap_flex_le; eauto. }
+      { esplits; eauto. econs. }
+      { esplits; eauto. econs. }
+    }
+    { ii. specialize (INHABITED loc).
+      eapply cap_flex_le in INHABITED; eauto.
+    }
+  Qed.
+
+  Lemma cap_left_end mem1 mem2 tm loc ts1 ts2 msg1
+        (MEM: Memory.closed mem1)
+        (CAP: cap_flex mem1 mem2 tm)
+        (GET: Memory.get loc ts2 mem1 = Some (ts1, msg1))
+    :
+      exists ts0 msg0,
+        (<<GET: Memory.get loc ts1 mem2 = Some (ts0, msg0)>>).
+  Proof.
+    destruct (Memory.get loc ts1 mem1) as [[ts0 msg0]|] eqn:GETORG.
+    { eapply cap_flex_le in GETORG; eauto. }
+    { hexploit (@cell_elements_greatest
+                  (mem1 loc)
+                  (fun ts => Time.lt ts ts1)). i. des; cycle 1.
+      { inv MEM. specialize (INHABITED loc).
+        hexploit EMPTY; eauto. intros TS.
+        destruct (Time.le_lt_dec ts1 Time.bot); ss. destruct l.
+        { exfalso. eapply Time.lt_strorder.
+          eapply TimeFacts.lt_le_lt; eauto. eapply Time.bot_spec. }
+        { inv H. clarify. }
+      }
+      hexploit CAP.(cap_flex_middle).
+      { econs.
+        { eapply GET0. }
+        { eapply GET. }
+        { eapply TimeFacts.lt_le_lt; eauto. eapply memory_get_ts_le; eauto. }
+        { i. destruct TS2.
+          { destruct (Memory.get loc ts mem1) eqn:GETTS; auto. destruct p.
+            eapply GREATEST in GETTS; eauto. timetac. }
+          { inv H. eauto. }
+        }
+      }
+      { auto. }
+      eauto.
+    }
+  Qed.
+
+End CAPFLEX.
